make greater equivalence own its view

Lp2lc/Active/Util.lean
@@ -100,18 +100,17 @@ class Lesser {VK} {base : UIdView VK} (VK2 : (v : VK base.UId) → Sort v)
 
 /-- Adds a lawful inverse to a widened read-only view. -/
 class Greater {VK} {base : UIdView VK} (VK2 : UIdU → Sort v)
-    (view : UIdView.Greater base VK2) where -- FIXME:  should remove `view` argument similar to Lesser
-  inv (outer : UIdEquiv base) (value : VK2 view.UId) : view.UId
-  rightInv : ∀ (outer : UIdEquiv base) (value : VK2 view.UId),
-    view.get (inv outer value) = value
-  leftInv : ∀ (outer : UIdEquiv base) (receipt : view.UId),
-    inv outer (view.get receipt) = receipt
+    extends UIdView.Greater base VK2 where
+  inv (outer : UIdEquiv base) (value : VK2 UId) : UId
+  rightInv : ∀ (outer : UIdEquiv base) (value : VK2 UId),
+    get (inv outer value) = value
+  leftInv : ∀ (outer : UIdEquiv base) (receipt : UId),
+    inv outer (get receipt) = receipt
 
 /-- Extends a base equivalence with lawful subtype metadata and supertype bridges. -/
 class Extendable {VK} (base : UIdView VK) extends UIdEquiv base where
   mkLesser (Tagging : VK base.UId → Sort u) : Lesser Tagging
-  mkGreater {VK2 : UIdU → Sort u}
-      (view : UIdView.Greater base VK2) : Greater VK2 view
+  mkGreater (VK2 : UIdU → Sort u) : Greater (base := base) VK2
 
 end UIdEquiv
 
